ipt_ports_andlist_compress_correct

Primitive_Matchers/IPPortIfaceSpace_Syntax.thy
@@ -15,8 +15,17 @@ text{*Primitive Match Conditions which only support interfaces, IPv4 addresses, 
 type_synonym ipt_ports = "(16 word \<times> 16 word) list"
 
 
-datatype ipportiface_rule_match = Src ipt_ipv4range | Dst ipt_ipv4range | IIface iface | OIface iface | Prot protocol | Src_Ports ipt_ports | Dst_Ports ipt_ports | Extra string
+datatype_new ipportiface_rule_match = Src ipt_ipv4range | Dst ipt_ipv4range | IIface iface | OIface iface | Prot protocol | 
+  is_Src_Ports: Src_Ports (src_ports_sel: ipt_ports) | 
+  is_Dst_Ports: Dst_Ports (dst_ports_sel: ipt_ports) | 
+  Extra string
 
+
+
+lemma wf_disc_sel_ipportiface_rule_match[simp]: 
+      "wf_disc_sel (is_Src_Ports, src_ports_sel) Src_Ports"
+      "wf_disc_sel (is_Dst_Ports, dst_ports_sel) Dst_Ports"
+  by(simp_all add: wf_disc_sel.simps)
 
 
 (*subsection{*Example Packet*}*)
