Simple_Firewall/SimpleFw_Compliance.thy
@@ -2,8 +2,12 @@ theory SimpleFw_Compliance
 imports SimpleFw_Semantics "../Primitive_Matchers/IPPortIfaceSpace_Matcher" "../Semantics_Ternary" "../Output_Format/Negation_Type_Matching" "../Bitmagic/Numberwang_Ln"
 begin
 
-fun ipv4_word_netmask_to_nattuple :: "(ipv4addr \<times> nat)  \<Rightarrow> ipt_ipv4range" where
-  "ipv4_word_netmask_to_nattuple (ip, n) = Ip4AddrNetmask (dotteddecimal_of_ipv4addr ip) n"
+fun ipv4_word_netmask_to_ipt_ipv4range :: "(ipv4addr \<times> nat) \<Rightarrow> ipt_ipv4range" where
+  "ipv4_word_netmask_to_ipt_ipv4range (ip, n) = Ip4AddrNetmask (dotteddecimal_of_ipv4addr ip) n"
+
+fun ipt_ipv4range_to_ipv4_word_netmask :: " ipt_ipv4range \<Rightarrow> (ipv4addr \<times> nat)" where
+  "ipt_ipv4range_to_ipv4_word_netmask (Ip4Addr ip_ddecim) = (ipv4addr_of_dotteddecimal ip_ddecim, 32)" | 
+  "ipt_ipv4range_to_ipv4_word_netmask (Ip4AddrNetmask ip_ddecim n) = (ipv4addr_of_dotteddecimal ip_ddecim, n)"
 
 (*do I need monads?*)
 fun negation_type_to_match_expr :: "('a \<Rightarrow> 'b) \<Rightarrow> 'a negation_type \<Rightarrow> 'b match_expr" where
@@ -13,8 +17,8 @@ fun negation_type_to_match_expr :: "('a \<Rightarrow> 'b) \<Rightarrow> 'a negat
 fun simple_match_to_ipportiface_match :: "simple_match \<Rightarrow> ipportiface_rule_match match_expr" where
   "simple_match_to_ipportiface_match \<lparr>iiface=iif, oiface=oif, src=sip, dst=dip, proto=p, sports=sps, dports=dps \<rparr> = 
     MatchAnd (Match (IIface iif)) (MatchAnd (Match (OIface oif)) 
-    (MatchAnd (negation_type_to_match_expr (\<lambda>x. Src (ipv4_word_netmask_to_nattuple x)) sip )
-    (MatchAnd (negation_type_to_match_expr (\<lambda>x. Dst (ipv4_word_netmask_to_nattuple x)) dip )
+    (MatchAnd (negation_type_to_match_expr (\<lambda>x. Src (ipv4_word_netmask_to_ipt_ipv4range x)) sip )
+    (MatchAnd (negation_type_to_match_expr (\<lambda>x. Dst (ipv4_word_netmask_to_ipt_ipv4range x)) dip )
     (MatchAnd (Match (Prot p))
     (MatchAnd (negation_type_to_match_expr (\<lambda>x. Src_Ports [x]) sps)
     (negation_type_to_match_expr (\<lambda>x. Dst_Ports [x]) dps)
@@ -24,8 +28,8 @@ fun simple_match_to_ipportiface_match :: "simple_match \<Rightarrow> ipportiface
 
 (*is this usefull?*)
 lemma xxx: "matches \<gamma> (simple_match_to_ipportiface_match \<lparr>iiface=iif, oiface=oif, src=sip, dst=dip, proto=p, sports=sps, dports=dps \<rparr>) a p \<longleftrightarrow> 
-      matches \<gamma> (alist_and ([Pos (IIface iif), Pos (OIface oif)] @ (NegPos_map (Src \<circ> ipv4_word_netmask_to_nattuple) [sip])
-        @ (NegPos_map (Dst \<circ> ipv4_word_netmask_to_nattuple) [dip]) @ [Pos (Prot p)]
+      matches \<gamma> (alist_and ([Pos (IIface iif), Pos (OIface oif)] @ (NegPos_map (Src \<circ> ipv4_word_netmask_to_ipt_ipv4range) [sip])
+        @ (NegPos_map (Dst \<circ> ipv4_word_netmask_to_ipt_ipv4range) [dip]) @ [Pos (Prot p)]
         @ (NegPos_map (\<lambda>x. Src_Ports [x]) [sps]) @ (NegPos_map (\<lambda>x. Dst_Ports [x]) [dps]))) a p"
 apply(simp add:)
 apply(cases sip)
@@ -39,7 +43,7 @@ apply(simp_all add: bunch_of_lemmata_about_matches)
 done
 
 (*TODO: smelly duplication*)
-lemma matches_Src_simple_match: "matches (ipportiface_matcher, \<alpha>) (negation_type_to_match_expr (\<lambda>x. ipportiface_rule_match.Src (ipv4_word_netmask_to_nattuple x)) ip) a p \<longleftrightarrow>
+lemma matches_Src_simple_match: "matches (ipportiface_matcher, \<alpha>) (negation_type_to_match_expr (\<lambda>x. ipportiface_rule_match.Src (ipv4_word_netmask_to_ipt_ipv4range x)) ip) a p \<longleftrightarrow>
   simple_match_ip ip (p_src p)"
 apply(cases ip)
  apply(rename_tac i_ip)
@@ -53,7 +57,7 @@ apply(rename_tac iip n)
 apply(simp add: matches_case_ternaryvalue_tuple split: ternaryvalue.split)
 apply(simp add: bunch_of_lemmata_about_matches bool_to_ternary_simps ipv4addr_of_dotteddecimal_dotteddecimal_of_ipv4addr)
 done
-lemma matches_Dst_simple_match: "matches (ipportiface_matcher, \<alpha>) (negation_type_to_match_expr (\<lambda>x. ipportiface_rule_match.Dst (ipv4_word_netmask_to_nattuple x)) ip) a p \<longleftrightarrow>
+lemma matches_Dst_simple_match: "matches (ipportiface_matcher, \<alpha>) (negation_type_to_match_expr (\<lambda>x. ipportiface_rule_match.Dst (ipv4_word_netmask_to_ipt_ipv4range x)) ip) a p \<longleftrightarrow>
   simple_match_ip ip (p_dst p)"
 apply(cases ip)
  apply(rename_tac i_ip)
@@ -89,5 +93,68 @@ apply(simp_all add: bunch_of_lemmata_about_matches eval_ternary_simps ternary_to
 apply(simp_all add: ports_to_set_singleton_simple_match_port)
 apply(auto simp add: matches_case_ternaryvalue_tuple bunch_of_lemmata_about_matches bool_to_ternary_simps split: ternaryvalue.split) (* oh dear, sorry for that *)
 done
+
+
+thm normalized_match.simps
+
+fun ipportiface_match_to_simple_match :: "ipportiface_rule_match match_expr \<Rightarrow> simple_match" where
+  "ipportiface_match_to_simple_match (Match (IIface iif)) = simple_match_any\<lparr> iiface := iif \<rparr>" |
+  "ipportiface_match_to_simple_match (Match (OIface oif)) = simple_match_any\<lparr> oiface := oif \<rparr>" |
+  "ipportiface_match_to_simple_match (Match (Src ip)) = simple_match_any\<lparr> src := Pos (ipt_ipv4range_to_ipv4_word_netmask ip) \<rparr>" |
+  "ipportiface_match_to_simple_match (Match (Dst ip)) = simple_match_any\<lparr> dst := Pos (ipt_ipv4range_to_ipv4_word_netmask ip) \<rparr>" |
+  "ipportiface_match_to_simple_match (Match (Prot p)) = simple_match_any\<lparr> proto := p \<rparr>"|
+  "ipportiface_match_to_simple_match (Match (Src_Ports ps)) = simple_match_any\<lparr> sports := Pos (0,0) \<rparr>"
+  (* hmm, port list (\<or>) to one port, creates multiple rules! need normalize_ports for match_Expr*)
+(*\<dots>*)
+
+
+
+(*TODO: Move?*)
+fun ipt_ports_negation_type_normalize :: "ipt_ports negation_type \<Rightarrow> ipt_ports" where
+  "ipt_ports_negation_type_normalize (Pos ps) = ps" |
+  "ipt_ports_negation_type_normalize (Neg ps) = br2l (bitrange_invert (l2br ps))"
+
+lemma ipt_ports_negation_type_normalize_correct:
+      "matches (ipportiface_matcher, \<alpha>) (negation_type_to_match_expr (Src_Ports) ps) a p \<longleftrightarrow>
+       matches (ipportiface_matcher, \<alpha>) (Match (Src_Ports (ipt_ports_negation_type_normalize ps))) a p"
+      "matches (ipportiface_matcher, \<alpha>) (negation_type_to_match_expr (Dst_Ports) ps) a p \<longleftrightarrow>
+       matches (ipportiface_matcher, \<alpha>) (Match (Dst_Ports (ipt_ports_negation_type_normalize ps))) a p"
+apply(case_tac [!] ps)
+apply(simp_all add: matches_case_ternaryvalue_tuple bunch_of_lemmata_about_matches bool_to_ternary_simps l2br_br2l ports_to_set_bitrange split: ternaryvalue.split)
+done
+
+(*todo: move*)
+value "primitive_extractor (is_Src_Ports, src_ports_sel) m"
+
+term fold
+(* [ [(1,2) \<or> (3,4)]  \<and>  [] ]*)
+definition ipt_ports_andlist_compress :: "ipt_ports list \<Rightarrow> ipt_ports" where
+  "ipt_ports_andlist_compress pss = br2l (fold (\<lambda>ps accu. (bitrange_intersection (l2br ps) accu)) pss bitrange_UNIV)"
+
+lemma ipt_ports_andlist_compress_correct: "ports_to_set (ipt_ports_andlist_compress pss) = \<Inter> set (map ports_to_set pss)"
+  proof -
+    { fix accu
+      have "ports_to_set (br2l (fold (\<lambda>ps accu. (bitrange_intersection (l2br ps) accu)) pss accu)) = (\<Inter> set (map ports_to_set pss)) \<inter> (ports_to_set (br2l accu))"
+        apply(induction pss arbitrary: accu)
+         apply(simp_all add: ports_to_set_bitrange l2br_br2l)
+        by fast
+    }
+    from this[of bitrange_UNIV] show ?thesis
+      unfolding ipt_ports_andlist_compress_def by(simp add: ports_to_set_bitrange l2br_br2l)
+  qed
+
+(**TODO: combine proofs to alist_and**)
+find_consts "'b list \<Rightarrow> 'a match_expr"
+
+
+fun ipt_ports_compress :: "ipt_ports negation_type list \<Rightarrow> ipt_ports" where
+  "ipt_ports_compress (ps#pss) = (ipt_ports_negation_type_normalize ps)"
+
+value "case primitive_extractor (is_Src_Ports, src_ports_sel) m 
+        of (spts, rst) \<Rightarrow> map (\<lambda>spt. (MatchAnd (Match (Src_Ports [spt]))) rst) (merge_ipt_ports spts)"
+
+fun normalize_ipt_ports :: "ipportiface_rule_match match_expr \<Rightarrow> ipportiface_rule_match match_expr list" where
+  "normalize_ipt_ports (Match (Src_Ports [])) = []" |
+  "normalize_ipt_ports (Match (Src_Ports (p#ps))) = []"
 
 end
