Primitive_Matchers/IPPortIfaceSpace_Matcher.thy
@@ -58,5 +58,4 @@ lemma ipportiface_matcher_SrcDst_Inter:
  done
 
 
-
 end
